Move things to better places

gol_rulesScript.sml
@@ -43,4 +43,64 @@ Proof
   Cases_on ‘b’ \\ fs []
 QED
 
+(* area of influence *)
+
+Definition infl_def: (* influence *)
+  infl s (i,j) ⇔ live_adj s i j ≠ 0 ∨ (i,j) ∈ s
+End
+
+Theorem infl_compose:
+  infl s ∩ infl t = ∅ ⇒
+  step (s ∪ t) = step s ∪ step t
+Proof
+  fs [EXTENSION,FORALL_PROD]
+  \\ rw [IN_DEF,infl_def,step_def]
+  \\ first_x_assum (qspecl_then [‘p_1’,‘p_2’] mp_tac)
+  \\ Cases_on ‘s (p_1,p_2)’ \\ fs [] \\ rw []
+  \\ fs [live_adj_def,IN_DEF]
+QED
+
+Theorem infl_thm:
+  (i,j) ∈ infl s ⇔
+    (i-1, j-1) ∈ s ∨ (i, j-1) ∈ s ∨ (i+1, j-1) ∈ s ∨
+    (i-1, j  ) ∈ s ∨ (i, j  ) ∈ s ∨ (i+1, j  ) ∈ s ∨
+    (i-1, j+1) ∈ s ∨ (i, j+1) ∈ s ∨ (i+1, j+1) ∈ s
+Proof
+  fs [IN_DEF,infl_def]
+  \\ Cases_on ‘s (i,j)’ \\ fs [live_adj_def]
+  \\ fs [AC DISJ_COMM DISJ_ASSOC]
+QED
+
+Theorem infl_mono:
+  x ⊆ y ⇒ infl x ⊆ infl y
+Proof
+  fs [infl_thm,SUBSET_DEF,FORALL_PROD]
+  \\ rw [] \\ fs []
+QED
+
+Theorem step_SUBSET_infl:
+  step s ⊆ infl s
+Proof
+  fs [step_def,SUBSET_DEF] \\ PairCases \\ fs [IN_step,infl_thm]
+  \\ strip_tac
+  \\ ‘live_adj s x0 x1 ≠ 0’ by (pop_assum mp_tac \\ IF_CASES_TAC \\ fs [])
+  \\ last_x_assum kall_tac
+  \\ fs [live_adj_def,IN_DEF]
+QED
+
+Theorem infl_union:
+  DISJOINT (infl s) (infl s') ⇒ infl (s ∪ s') = infl s ∪ infl s'
+Proof
+  fs [EXTENSION,IN_DISJOINT,FORALL_PROD] \\ rw []
+  \\ eq_tac \\ fs [infl_thm]
+  THEN1 (rw [] \\ fs [])
+  \\ CCONTR_TAC \\ fs [] \\ res_tac \\ fs []
+QED
+
+(* list to set *)
+
+Definition to_state_def:
+  to_state xs = { p | MEM (p,T) xs } : state
+End
+
 val _ = export_theory();
